bound/UpperBound_A.v
@@ -822,6 +822,7 @@ Section PRESERVATION.
       destruct frs_tgt; ss.
       { exploit match_stacks_right_nil; et. i; des. clarify. }
       rename t into fr_tgt.
+      ii. clear SSSRC SSTGT.
       destruct (classic (fr_tgt.(Frame.ms).(ModSem.is_call) fr_tgt.(Frame.st))).
       (* tgt call *)
       (* fsim *)
@@ -1527,7 +1528,7 @@ i. des_safe. inv H0. unfold is_call_cont_strong. auto. }
             exploit preservation_cp_focus; eauto. }
           exploit match_stacks_focus; eauto. }
     (* call state *)
-    - right. econs; ss; et.
+    - right. clear SSSRC SSTGT. econs; ss; et.
       i.
       econs; cycle 1.
       { i. specialize (SAFESRC _ (star_refl _ _ _ _)). des; ss.
@@ -1595,7 +1596,7 @@ i. des_safe. inv H0. unfold is_call_cont_strong. auto. }
   Theorem upperbound_a_xsim :
       <<XSIM: mixed_simulation (Sem.sem prog_src) (Sem.sem prog_tgt)>>.
   Proof.
-    econs; ss; eauto. econs; try apply progress_top; ss; eauto.
+    econs; ss; eauto. econs; try apply preservation_top; ss; eauto.
     { eapply unit_ord_wf. }
     { econs 1.
       ii. inversion INITSRC. exploit init_fsim; eauto. i; des. esplits; eauto.
@@ -1624,7 +1625,7 @@ Proof.
   eapply mixed_to_backward_simulation.
   destruct (link_sk (ctx ++ [module cp_link])) eqn:LINKSK; cycle 1.
   { econs; et.
-    econs; try apply progress_top; et.
+    econs; try apply preservation_top; et.
     { eapply unit_ord_wf. }
     { econs; et. i. ss. inv INITSRC. clarify. }
     i; des. ss. des_ifs.
