bound/UpperBound_B.v
@@ -1281,7 +1281,7 @@ Section PRESERVATION.
                     subst. ss. }
                 exploit Genv.find_funct_inversion; eauto. i; des. f_equal.
                 inv WTPROG. exploit CSTYLE_EXTERN; eauto. i. des_ifs. f_equal. eapply H3; eauto. }
-              { inv SSSRC; ss. exploit WTKS; eauto. { ii. clarify. } esplits; ss; eauto. rr. des. des_ifs. }
+              { specialize (SSSRC _ _ (star_refl _ _ _ _)). inv SSSRC; ss. exploit WTKS; eauto. { ii. clarify. } esplits; ss; eauto. rr. des. des_ifs. }
              (* internal *)
              ++ exploit progress_step; eauto.
         * inv MTCHST.
@@ -1292,36 +1292,40 @@ Section PRESERVATION.
           { inv INITTGT. }
   Qed.
 
+  Hypothesis INITSAFE: forall st (INIT: Smallstep.initial_state (semantics prog) st),
+      <<SAFE: safe (semantics prog) st>>.
+
   Lemma transf_xsim_properties:
       xsim_properties (Csem.semantics prog) (Sem.sem tprog) nat lt.
   Proof.
-    econstructor 1 with (ss_src := wt_state prog ge) (ss_tgt := top1);
-      ss; [| |apply lt_wf| |i; apply symb_preserved].
-    { clear - MAIN_INTERNAL tprog WTPROG SKEWF LINK_SK_TGT.
-      ii. inv INIT.
-      destruct (classic (exists fd, Genv.find_funct (globalenv prog) (Vptr b Ptrofs.zero) = Some (Internal fd))).
-      - eapply wt_initial_state; ss; eauto.
-        { i. rr. rewrite Genv.find_def_symbol. esplits; eauto. }
-        { des. ii.
-          destruct SKEWF.
-          destruct match_ge_skenv_link.
-          specialize (mge_defs blk). inv mge_defs.
-          { ss. unfold Genv.find_def in DEF. unfold fundef, genv_genv in *. ss.
-            symmetry in H5. Eq. }
-          ss. unfold Genv.find_def in DEF. unfold fundef, genv_genv in *. ss.
-          symmetry in H4. Eq.
-          symmetry in H5. exploit DEFSYMB; eauto. i. des.
-          unfold Genv.find_symbol in *. rewrite mge_symb in H4. eauto. }
-      - ss. des_ifs.
-        specialize (SAFE _ (star_refl _ _ _ _)). des; inv SAFE; ss.
-        { inv H4. }
-        { contradict H3. inv H4; ss; des_ifs; rewrite FPTR in *; eauto.
-          exploit MAIN_INTERNAL; eauto.
-          { econs; eauto. }
-          i; des. ss. des_ifs.
-        }
+    econstructor 1 with (xsim_ss_src := wt_state prog ge) (xsim_ss_tgt := top1);
+      ss; [|apply lt_wf| |i; apply symb_preserved].
+    { clear - MAIN_INTERNAL tprog WTPROG SKEWF LINK_SK_TGT INITSAFE WTSK WT_EXTERNAL INCL.
+      econs.
+      - ii. hexploit INITSAFE; eauto. intro SAFE. inv INIT.
+        destruct (classic (exists fd, Genv.find_funct (globalenv prog) (Vptr b Ptrofs.zero) = Some (Internal fd))).
+        + eapply wt_initial_state; ss; eauto.
+          { i. rr. rewrite Genv.find_def_symbol. esplits; eauto. }
+          { des. ii.
+            destruct SKEWF.
+            destruct match_ge_skenv_link.
+            specialize (mge_defs blk). inv mge_defs.
+            { ss. unfold Genv.find_def in DEF. unfold fundef, genv_genv in *. ss.
+              symmetry in H5. Eq. }
+            ss. unfold Genv.find_def in DEF. unfold fundef, genv_genv in *. ss.
+            symmetry in H4. Eq.
+            symmetry in H5. exploit DEFSYMB; eauto. i. des.
+            unfold Genv.find_symbol in *. rewrite mge_symb in H4. eauto. }
+        + ss. des_ifs.
+          specialize (SAFE _ (star_refl _ _ _ _)). des; inv SAFE; ss.
+          { inv H4. }
+          { contradict H3. inv H4; ss; des_ifs; rewrite FPTR in *; eauto.
+            exploit MAIN_INTERNAL; eauto.
+            { econs; eauto. }
+            i; des. ss. des_ifs.
+          }
+      - ii. eapply preservation_prog; eauto. rewrite <- senv_same; et.
     }
-    { ii. eapply preservation_prog; eauto. rewrite <- senv_same; et. }
     econs. i.
     exploit (transf_initial_states); eauto.
     i. des. esplits. econs; eauto.
@@ -1376,6 +1380,7 @@ Proof.
           + exploit IHl; eauto.
         - split; unfold link_sk, link_list in *; ss; unfold link_prog in *; des_ifs. }
       rewrite T2 in H0. clarify. }
+  eapply improves_free_theorem; i.
   eapply bsim_improves.
   eapply mixed_to_backward_simulation.
   inv TYPED.
