common/BehaviorsC.v
@@ -34,3 +34,57 @@ Proof.
   eapply backward_to_compcert_backward_simulation; eauto.
 Qed.
 
+Lemma back_propagate_ub_behav
+      beh0
+      (INITUB: behavior_improves beh0 (Goes_wrong E0)):
+    <<INITUB: beh0 = Goes_wrong E0>>.
+Proof.
+  rr in INITUB. des; clarify; et.
+  rr in INITUB0. des. unfold behavior_app in *. des_ifs. destruct t; ss.
+Qed.
+
+Lemma back_propagate_ub_program
+      sem0 sem1
+      (IMPR: improves sem0 sem1)
+      (INITUB: program_behaves sem1 (Goes_wrong E0)):
+    <<INITUB: program_behaves sem0 (Goes_wrong E0)>>.
+Proof.
+  exploit IMPR; eauto. i; des.
+  hexploit back_propagate_ub_behav; et. i ;des. clarify.
+Qed.
+
+Lemma improves_free_theorem
+      L1 L2
+      (IMPRV: forall
+          (INITSAFE: exists st, <<INIT: Smallstep.initial_state L1 st>>)
+          (INITSAFE: forall st (INIT: Smallstep.initial_state L1 st),
+              <<SAFE: safe L1 st>>)
+        ,
+          improves L1 L2)
+  :
+    <<IMPRV: improves L1 L2>>
+.
+Proof.
+  destruct (classic (exists st, <<INIT: Smallstep.initial_state L1 st>>)); cycle 1.
+  { clear - H.
+    ii.
+    exists (Goes_wrong []). esplits; ss; eauto using behavior_improves_bot.
+    econs 2; eauto.
+  }
+  destruct (classic (forall st (INIT: Smallstep.initial_state L1 st), <<SAFE: safe L1 st>>)); cycle 1.
+  { clear - H0. rename H0 into H.
+    ii.
+    exists (Goes_wrong []). esplits; ss; eauto.
+    - apply Classical_Pred_Type.not_all_ex_not in H. des.
+      apply Classical_Prop.imply_to_and in H. des.
+      econs 1; eauto.
+      clear - H0.
+      apply Classical_Pred_Type.not_all_ex_not in H0. des.
+      repeat (apply_all_once Classical_Prop.imply_to_and; des).
+      apply Classical_Prop.not_or_and in H1. des.
+      econs 4; eauto.
+      ii. eapply H2; eauto.
+    - eapply behavior_improves_bot; eauto.
+  }
+  eauto.
+Qed.
